Working on sequencing

Safety.v
@@ -1,17 +1,68 @@
 From Coq Require Import Init.Nat.
 
+From Elo Require Export Array.
+From Elo Require Export Map.
+
 From Elo Require Export Core.
+From Elo Require Export Properties.
 
+Reserved Notation "m / ths '==[' f ']==>+' m' / ths'"
+  (at level 40, ths at next level, f at next level, m' at next level).
 
-Inductive sequence : nat -> ceffect -> mem -> list tm -> Prop :=
-  | sequence_nil : forall m th,
-    sequence 0 (CEF_None 0) m (th :: nil)
+Inductive multistep (f : ceffect -> Prop) :
+  mem -> list tm -> mem -> list tm -> Prop :=
 
-  | sequence_cons : forall i m m' ths ths' eff eff',
-    sequence i eff m ths ->
-    m / ths ==> m' / ths' # eff' ->
-    sequence (S i) eff' m' ths'
+  | multistep_first : forall m m' ths ths' ceff,
+    f ceff ->
+    m / ths ==> m' / ths' # ceff ->
+    m / ths ==[f]==>+ m' / ths'
+
+  | multistep_step : forall m1 m m2 ths1 ths ths2 ceff,
+    f ceff ->
+    m1 / ths1 ==> m / ths # ceff ->
+    m  / ths  ==[f]==>+ m2 / ths2 ->
+    m1 / ths1 ==[f]==>+ m2 / ths2
+
+  where "m / ths '==[' f ']==>+' m' / ths'" := (multistep f m ths m' ths').
+
+Reserved Notation "m / ths '==[' f ']==>+' m' / ths'"
+  (at level 40, ths at next level, f at next level, m' at next level).
+
+Inductive sequence : list ceffect -> mem -> list tm -> Prop :=
+  | sequence_nil : forall main,
+    sequence (CEF_None 0 :: nil) nil (main :: nil)
+
+  | sequence_cons : forall m m' ths ths' ceff ceffs,
+    m / ths ==> m' / ths' # ceff ->
+    sequence ceffs  m  ths ->
+    sequence (ceff :: ceffs) m' ths'
   .
+
+Definition is_same_thread ceff i :=
+  match ceff with
+  | CEF_None  j
+  | CEF_Alloc j _
+  | CEF_Load  j _
+  | CEF_Store j _
+  | CEF_Spawn j   => i =? j
+  end.
+
+Definition is_write ceff addr :=
+  match ceff with
+  | CEF_Store _ addr' => addr =? addr'
+  | _ => false
+  end.
+
+Definition is_not_concurrent_write (i addr : nat) (ceff : ceffect) :=
+  False.
+
+Theorem aux : forall m1 m2 m3 ths1 ths2 ths3 i addr,
+  m1 / ths1 ==> m2 / ths2 # (CEF_Load i addr) ->
+  m2 / ths2 ==[is_not_concurrent_write i addr]==>+ m3 / ths3.
+Proof.
+Admitted.
+
+
 
 Inductive before : list tm -> list tm -> Prop :=
   | todo : forall i j eff eff' m m' ths ths',
@@ -25,12 +76,6 @@ Definition synchronize (threads : list tm) (i j : nat) : Prop := False.
 
 Definition happens_before (threads : list tm) i j : Prop :=
   if i =? j then i < j else synchronize threads i j.
-
-Definition is_write (t : tm) : Prop := 
-  match t with
-  | TM_Asg _ _ | TM_ArrAsg _ _ _ => True
-  | _ => False
-  end.
 
 Definition data_race := forall (threads : list tm) i j,
   (is_write (get_tm threads i) \/ is_write (get_tm threads j)) /\
